Homework

teaching/taltech2019/ex/hw/FileSystem.fst
@@ -11,10 +11,17 @@ module FileSystem
   asked to equip the `show`, `create_dir`, and `delete` functions with 
   strong specifications and prove that your implementations satisfy them.
 
-  The exercise is divided into 6 tasks---see below for further details.
+  The exercise is divided into 7 tasks---see below for further details. 
+  The tasks are somewhat independent. For instance, you can either first
+  implement the file system operations (Tasks 4-6) and then strengthen 
+  their specifications (Task 7); or you can first try to come up with 
+  suitably strong specifications for them to verify `FileSystemClient.fst`
+  (Task 7) and only afterwards try to come up with real implementations 
+  that would also satisfy these stronger specifications.
 
   When solving the tasks below, do not be afraid of defining additional 
-  auxiliary (pure) recursive functions and use them in the specifications.
+  auxiliary (pure) recursive functions, state and prove lemmas about 
+  these functions, and then use them in the various specifications.
 
 *)
 
@@ -36,7 +43,7 @@ type path = p:list string{True}
 type fs_tree =
   | Node : list (string * fs_tree) -> fs_tree
 
-(* An effect that characterises programs that use the file system. *)
+(* A (monadic) effect that characterises programs that use a file system. *)
 
 let fs_st (a:Type) = fs_tree -> M (a * fs_tree)
 
@@ -71,14 +78,14 @@ total new_effect {
           
 *)
 
-let fs_tree_wf (fs:fs_tree) : bool = 
+let fs_tree_wf (fs:fs_tree) : Type0 = 
   admit ()
 
 let wf_fs_tree = fs:fs_tree{fs_tree_wf fs}
 
 (* Pre- and postcondition variant of the `FileSystem` effect, which additionally 
    assumes that the initial file system (`fs0`) is well-formed and additionally 
-   requires one to prove that the final file system (`fs1`) is still well-formed. *)
+   requires one to prove that the final file system (`fs1`) remains well-formed. *)
 
 effect FS (a:Type) 
           (pre:wf_fs_tree -> Type0) 
@@ -100,18 +107,21 @@ let write (fs:wf_fs_tree) : FS unit
                                (ensures  (fun _ _ fs1 -> fs1 == fs)) = 
   FileSystem?.write fs
 
+(*
+
+   Task 3: Define a predicate that holds if a given path exists in a given file system.
+
+*)
+
+let in_fs (p:path) (fs:wf_fs_tree) : Type = 
+  admit ()
 
 (* 
 
-  Task 3: Define a pure function that returns all the paths in a given file system. 
-          Also, define a function in the the `FS` effect that returns all paths in 
-          the current state of the file system.
-
+  Task 4: Define a function in the the `FS` effect that returns all paths in the file system.
+        
 *)
            
-let show_fs (fs:fs_tree) : list path =
-  admit ()
-
 let show () : FS (list path)
                  (requires (fun fs0 -> True)) 
                  (ensures  (fun fs0 ps fs1 -> True)) =
@@ -119,7 +129,7 @@ let show () : FS (list path)
 
 (* 
 
-  Task 4: Define a function in the `FS` effect that creates a new directory in the file system. 
+  Task 5: Define a function in the `FS` effect that creates a new directory in the file system. 
 
   Hint: As part of defining `create_dir`, you also need to prove that creating a well-formed 
         path in a well-formed tree results in a well-formed tree. 
@@ -133,7 +143,7 @@ let create_dir (p:path) : FS unit
 
 (* 
 
-  Task 5: Define a function in the `FS` effect that deletes a given path from the file system. 
+  Task 6: Define a function in the `FS` effect that deletes a given path from the file system. 
 
   Hint: As part of defining `delete`, you also need to prove that deleting a well-formed path 
         from a well-formed tree results in a well-formed tree. 
@@ -147,12 +157,18 @@ let delete (p:path) : FS unit
 
 (* 
 
-  Task 6: Strengthen the (currently trivial) specifications of `show`, `create_dir`, and
+  Task 7: Strengthen the (currently trivial) specifications of `show`, `create_dir`, and
           `delete` so that the test code in `FileSystemClient.fst` successfully typechecks. 
                
-  Hint: Think about the resulting shape of the file system after creating a new path in it or 
-        removing an already existing path. You can draw inspiration from the `deleteDeletes`
-        and `createAndDelete` FSCheck properties you defined in your regular coursework. 
-        Similarly, the list of paths returned by `show` is not any old list of paths. 
-        
+  Hint 1: Think about the resulting shape of the file system after creating a new path in it or 
+          removing an already existing path. You can draw inspiration from the `deleteDeletes`
+          and `createAndDelete` FSCheck properties you defined in your regular coursework. 
+          Similarly, the list of paths returned by `show` is not any old list of paths. 
+
+  Hint 2: Do not be afraid of defining auxiliary pure functions (using the default `Tot` effect)
+          which you can then use as part of the specifications. Most probably you will also
+          need to state and prove some lemmas about these functions (using the `Lemma` effect), 
+          e.g., so as to relate the spec of `create_dir` to the spec of `delete` if one follows 
+          the other in user code (as in FileSystemClient.fst).
+
 *)
