teaching/taltech2019/ex/hw/FileSystemClient.fst
@@ -4,7 +4,10 @@ module FileSystemClient
 
    Homework exercise.
 
-   See `FileSystem.fst` for details.
+   See `FileSystem.fst` for further details about this exercise.
+
+   Below you can uncomment the `expect_failure` attributes in case
+   you want to first make some of the the latter tests typecheck.
 
 *)
 
@@ -12,29 +15,43 @@ open FileSystem
 
 open FStar.List.Tot
 
-let test1 (p:path) : FS unit
+//[@expect_failure]
+let test1 (p:path) : FS unit 
+                        (requires (fun fs0 -> fs0 == Node []))
+                        (ensures  (fun fs0 _ fs1 -> fs0 == fs1)) =
+  create_dir p;
+  delete p
+
+//[@expect_failure]
+let test2 (p:path) : FS unit
                         (requires (fun fs0 -> fs0 == Node []))
                         (ensures  (fun fs0 _ fs1 -> fs0 == fs1)) =
   create_dir p;
   let _ = show () in
   delete p
 
-let test2 (p:path) : FS (list path)
+//[@expect_failure]
+let test2' (p:path) : FS unit
+                         (requires (fun fs0 -> True))
+                         (ensures  (fun fs0 _ fs1 -> in_fs p fs1)) =
+  create_dir p
+
+//[@expect_failure]
+let test2'' (p:path) : FS unit
+                         (requires (fun fs0 -> True))
+                         (ensures  (fun fs0 _ fs1 -> ~(in_fs p fs1))) =
+  delete p
+
+//[@expect_failure]
+let test3 (p:path) : FS (list path)
                         (requires (fun fs0 -> fs0 == Node []))
-                        (ensures  (fun fs0 ps fs1 -> 
-                                     count p ps == 1 /\
-                                     fs0 == fs1)) =
+                        (ensures  (fun fs0 ps fs1 -> mem p ps /\ fs0 == fs1)) =
   create_dir p;
   let ps = show () in
   delete p;
   ps
 
-let test3 (p:path) : FS unit 
-                        (requires (fun fs0 -> fs0 == Node []))
-                        (ensures  (fun fs0 _ fs1 -> fs0 == fs1)) =
-  create_dir p;
-  delete p
-
+//[@expect_failure]
 let test4 (p1 p2 p3:path) : FS unit 
                                (requires (fun fs0 -> fs0 == Node []))
                                (ensures  (fun fs0 _ fs1 -> fs0 == fs1)) =
@@ -45,18 +62,16 @@ let test4 (p1 p2 p3:path) : FS unit
   delete p2;
   delete p3
 
+//[@expect_failure]
 let test5 (p1 p2:path) : FS unit
                         (requires (fun fs0 -> True))
-                        (ensures  (fun _ _ fs1 -> 
-                                    count p1 (show_fs fs1) == 1 /\ 
-                                    count p2 (show_fs fs1) == 1)) =
+                        (ensures  (fun _ _ fs1 -> in_fs p1 fs1 /\ in_fs p2 fs1)) =
   create_dir p1;
   create_dir p2
 
+//[@expect_failure]
 let test6 (p1 p2:path) : FS unit
                             (requires (fun fs0 -> True))
-                            (ensures  (fun _ _ fs1 -> 
-                                        count p1 (show_fs fs1) == 0 /\ 
-                                        count p2 (show_fs fs1) == 0)) =
+                            (ensures  (fun _ _ fs1 -> ~(in_fs p1 fs1) /\ ~(in_fs p2 fs1))) =
   delete p1;
   delete p2
